progress on phase one top-down proof

systems/ChordCorrectness.v
@@ -1,4 +1,9 @@
 Require Import List.
+Import ListNotations.
+Require Import Omega.
+
+Require Verdi.Coqlib.
+Require Import StructTact.StructTactics.
 
 Require Import Chord.Chord.
 Import Chord.Chord.Chord.
@@ -8,9 +13,125 @@ Require Import Chord.ChordSemantics.
 Import ChordSemantics.
 Import ConstrainedChord.
 
+Set Bullet Behavior "Strict Subproofs".
+Open Scope nat_scope.
+
+Definition reachable_after_churn gst :=
+  exists ex,
+    reachable_st (occ_gst (infseq.hd ex)) /\
+    lb_execution ex /\
+    infseq.eventually (fun ex' => gst = (occ_gst (infseq.hd ex'))) ex.
+
+Definition live_addr (gst : global_state) (a : addr) :=
+  In a (nodes gst) /\
+  ~ In a (failed_nodes gst) /\
+  exists st, sigma gst a = Some st.
+
+Lemma live_node_is_live_addr :
+  forall gst h,
+    live_node gst h ->
+    live_addr gst h.
+Proof.
+  intros.
+  unfold live_addr.
+  repeat split;
+    eauto using live_node_joined,
+                live_node_in_nodes,
+                live_node_not_in_failed_nodes,
+                live_node_means_state_exists.
+Qed.
+
 Definition live (gst : global_state) (p : pointer) :=
-  In (addr_of p) (nodes gst) /\
-  ~ In (addr_of p) (failed_nodes gst).
+  live_addr gst (addr_of p).
+
+Lemma live_live_addr :
+  forall gst p,
+    live gst p <-> live_addr gst (addr_of p).
+Proof.
+  now unfold live.
+Qed.
+
+Lemma live_addr_intro :
+  forall gst a st,
+    In a (nodes gst) ->
+    ~ In a (failed_nodes gst) ->
+    sigma gst a = Some st ->
+    live_addr gst a.
+Proof.
+  unfold live_addr.
+  eauto.
+Qed.
+
+Lemma live_intro :
+  forall gst p st,
+    In (addr_of p) (nodes gst) ->
+    ~ In (addr_of p) (failed_nodes gst) ->
+    sigma gst (addr_of p) = Some st ->
+    live gst p.
+Proof.
+  unfold live.
+  eauto using live_addr_intro.
+Qed.
+
+Lemma live_addr_inv :
+  forall gst a,
+    live_addr gst a ->
+    In a (nodes gst) /\
+    ~ In a (failed_nodes gst) /\
+    exists st, sigma gst a = Some st.
+Proof.
+  easy.
+Qed.
+
+Lemma live_inv :
+  forall gst p,
+    live gst p ->
+    In (addr_of p) (nodes gst) /\
+    ~ In (addr_of p) (failed_nodes gst) /\
+    exists st, sigma gst (addr_of p) = Some st.
+Proof.
+  easy.
+Qed.
+
+Ltac live_addr_inv :=
+  match goal with
+  | [ H_live : live_addr ?gst ?a |- _ ] =>
+    apply live_addr_inv in H_live;
+      destruct H_live as [?H [?H ?H]];
+      match goal with
+      | [ H_st : exists st, sigma gst a = Some st |- _ ] =>
+        destruct H_st as [?st]
+      end
+  end.
+
+Ltac live_inv :=
+  match goal with
+  | [ H_live : live ?gst ?p |- _ ] =>
+    apply live_inv in H_live;
+      destruct H_live as [?H [?H ?H]];
+      match goal with
+      | [ H_st : exists st, sigma gst (addr_of p) = Some st |- _ ] =>
+        destruct H_st as [?st]
+      end
+  end.
+
+Definition live_addr_dec :
+  forall gst a,
+    {live_addr gst a} + {~ live_addr gst a}.
+Admitted.
+
+Definition live_nodes (gst : global_state) : list addr :=
+  filter (fun a => Coqlib.proj_sumbool
+                  (live_addr_dec gst a))
+         (nodes gst).
+
+Definition live_nodes_with_states (gst : global_state) : list (addr * data) :=
+  FilterMap.filterMap (fun a =>
+         match sigma gst a with
+         | Some st => Some (a, st)
+         | None => None
+         end)
+      (live_nodes gst).
 
 Definition correct_succs
            (gst : global_state)
@@ -25,8 +146,6 @@ Definition correct_succs
 Definition full_succs (gst : global_state) (h : pointer) (succs : list pointer) : Prop :=
   length succs = Chord.SUCC_LIST_LEN.
 
-Print best_succ.
-
 (* cf. zave page 11 *)
 Definition first_succ_is_best_succ (gst : global_state) (h : addr) :=
   exists st s rest,
@@ -39,17 +158,368 @@ Definition all_first_succs_best (gst : global_state) :=
     live gst h ->
     first_succ_is_best_succ gst (addr_of h).
 
-Definition eventually_always_net
-           (P : global_state -> Prop) : infseq.infseq occurrence -> Prop :=
-  infseq.eventually
-    (infseq.always
-       (fun ex' => P (occ_gst (infseq.hd ex')))).
+Definition gpred_and (P Q : global_state -> Prop) (gst : global_state) : Prop :=
+  P gst /\ Q gst.
+
+Definition lift_gpred_to_ex (P : global_state -> Prop) (ex : infseq.infseq occurrence) :=
+  P (occ_gst (infseq.hd ex)).
 
 Definition phase_one (ex : infseq.infseq occurrence) :=
   lb_execution ex ->
   reachable_st (occ_gst (infseq.hd ex)) ->
-  eventually_always_net all_first_succs_best ex.
- 
+  infseq.continuously (lift_gpred_to_ex all_first_succs_best) ex.
+
+(* Defining the error for phase one: the norm approach *)
+Fixpoint succ_list_leading_failed_nodes (failed : list addr) (succs : list pointer) : nat :=
+  match succs with
+  | h :: rest =>
+    if In_dec addr_eq_dec (addr_of h) failed
+    then S (succ_list_leading_failed_nodes failed rest)
+    else 0
+  | [] => 0
+  end.
+
+Definition sum (l : list nat) :=
+  fold_left Nat.add l 0.
+
+Definition maybe_count_failed_nodes (gst : global_state) (h : addr) :=
+  match sigma gst h with
+  | Some st =>
+    Some (succ_list_leading_failed_nodes (failed_nodes gst) (succ_list st))
+  | None =>
+    None
+  end.
+
+Lemma maybe_count_failed_nodes_Some :
+  forall gst h st n,
+    maybe_count_failed_nodes gst h = Some n ->
+    sigma gst h = Some st ->
+    succ_list_leading_failed_nodes (failed_nodes gst) (succ_list st) = n.
+Proof.
+  unfold maybe_count_failed_nodes.
+  intros.
+  break_match; congruence.
+Qed.
+
+Definition total_leading_failed_nodes (gst : global_state) : nat :=
+  sum (FilterMap.filterMap (maybe_count_failed_nodes gst) (live_nodes gst)).
+
+Definition nonempty_succ_lists (gst : global_state) : Prop :=
+  forall h st,
+    sigma gst h = Some st ->
+    succ_list st <> [].
+
+Lemma equal_folds_means_equal_acc :
+  forall l a b,
+    fold_left Nat.add l a = fold_left Nat.add l b ->
+    a = b.
+Proof.
+  unfold sum.
+  induction l.
+  - easy.
+  - simpl.
+    intros.
+    find_apply_hyp_hyp.
+    omega.
+Qed.
+
+Lemma fold_left_acc_comm :
+  forall a l,
+    fold_left Nat.add l a = a + fold_left Nat.add l 0.
+Proof.
+  intros.
+  generalize a.
+  induction l.
+  - easy.
+  - simpl.
+    intros.
+    rewrite (IHl (_ + _)).
+    rewrite (IHl a0).
+    omega.
+Qed.
+
+(* TODO(ryan) move to structtact *)
+Theorem list_strong_ind :
+  forall A (P : list A -> Prop),
+    (forall l, (forall l', length l' < length l -> P l') ->
+        P l) ->
+    forall l0 : list A, P l0.
+Proof.
+  intros.
+  apply H.
+  induction l0; simpl.
+  - intros.
+    now find_apply_lem_hyp Nat.nlt_0_r.
+  - intros.
+    apply H; intros.
+    intuition eauto using lt_n_Sm_le, lt_le_trans.
+Qed.
+
+Lemma sum_of_nats_bounds_addends :
+  forall l n,
+    sum l = n ->
+    forall x,
+      In x l ->
+      x <= n.
+Proof.
+  unfold sum.
+  intro l.
+  induction l using list_strong_ind.
+  destruct l.
+  - easy.
+  - intros.
+    find_apply_lem_hyp in_inv. break_or_hyp.
+    + simpl.
+      rewrite fold_left_acc_comm.
+      omega.
+    + simpl. rewrite fold_left_acc_comm.
+      assert (x <= fold_left Nat.add l 0).
+      { assert (H_len: length l < length (n :: l)) by auto.
+        apply (H l H_len); auto.
+      }
+      omega.
+Qed.
+
+Lemma sum_of_nats_zero_means_all_zero :
+  forall l,
+    sum l = 0 ->
+    forall x,
+      In x l ->
+      x = 0.
+Proof.
+  intros.
+  symmetry.
+  apply le_n_0_eq.
+  eapply sum_of_nats_bounds_addends; eauto.
+Qed.
+
+Definition successor_nodes_valid (gst : global_state) : Prop :=
+  forall h p st,
+    In p (succ_list st) ->
+    sigma gst h = Some st ->
+    In (addr_of p) (nodes gst) /\
+    exists pst, sigma gst (addr_of p) = Some pst /\
+           joined pst = true.
+
+Lemma successor_nodes_valid_state :
+  forall gst h p st,
+    In p (succ_list st) ->
+    successor_nodes_valid gst ->
+    sigma gst h = Some st ->
+    exists pst, sigma gst (addr_of p) = Some pst /\
+           joined pst = true.
+Proof.
+  intros.
+  eapply_prop_hyp successor_nodes_valid @eq; eauto.
+  now break_and.
+Qed.
+
+Lemma successor_nodes_valid_inv :
+  forall gst h p st,
+    In p (succ_list st) ->
+    successor_nodes_valid gst ->
+    sigma gst h = Some st ->
+    In (addr_of p) (nodes gst) /\
+    exists pst, sigma gst (addr_of p) = Some pst /\
+           joined pst = true.
+Proof.
+  eauto.
+Qed.
+
+Lemma successor_nodes_valid_live_are_joined :
+  forall gst h st p,
+    live gst p ->
+    successor_nodes_valid gst ->
+    sigma gst h = Some st ->
+    In p (succ_list st) ->
+    live_node gst (addr_of p).
+Proof.
+  intros.
+  live_inv.
+  find_eapply_lem_hyp successor_nodes_valid_inv;
+    eauto; repeat (break_and; break_exists).
+  eapply live_node_characterization; eauto.
+Qed.
+
+Lemma successor_nodes_always_valid :
+  forall gst,
+    reachable_after_churn gst ->
+    successor_nodes_valid gst.
+Proof.
+Admitted.
+
+Lemma nonempty_succ_lists_always_belong_to_joined_nodes :
+  forall gst h st,
+    reachable_after_churn gst ->
+    sigma gst h = Some st ->
+    succ_list st <> [] ->
+    joined st = true.
+Admitted.
+
+Lemma zero_leading_failed_nodes_leading_node_live :
+  forall gst h st s rest,
+    succ_list_leading_failed_nodes (failed_nodes gst) (succ_list st) = 0 ->
+    reachable_after_churn gst ->
+    sigma gst h = Some st ->
+    succ_list st = s :: rest ->
+    live gst s.
+Proof.
+  intros.
+  repeat find_rewrite.
+  simpl in *.
+  break_if; try congruence.
+  unfold succ_list_leading_failed_nodes.
+  find_apply_lem_hyp successor_nodes_always_valid.
+  assert (In s (succ_list st)).
+  {
+    find_rewrite.
+    apply in_eq.
+  }
+  find_eapply_lem_hyp successor_nodes_valid_inv; eauto; repeat (break_exists_name pst || break_and).
+  eapply live_intro; eauto.
+Qed.
+
+Lemma zero_leading_failed_nodes_best_succ :
+  forall gst h st s rest,
+    succ_list_leading_failed_nodes (failed_nodes gst) (succ_list st) = 0 ->
+    reachable_after_churn gst ->
+    sigma gst h = Some st ->
+    succ_list st = s :: rest ->
+    live_node gst h ->
+    best_succ gst h (addr_of s).
+Proof.
+  unfold best_succ.
+  intros.
+  exists st.
+  exists [].
+  exists (map addr_of rest).
+  simpl.
+  intuition.
+  - repeat find_rewrite.
+    apply map_cons.
+  - eapply successor_nodes_valid_live_are_joined; eauto.
+    + find_copy_eapply_lem_hyp zero_leading_failed_nodes_leading_node_live; eauto.
+    + apply successor_nodes_always_valid.
+      assumption.
+    + repeat find_rewrite.
+      apply in_eq.
+Qed.
+
+Lemma zero_failed_nodes_total_implies_zero_locally :
+  forall gst h st,
+    total_leading_failed_nodes gst = 0 ->
+    live_addr gst h ->
+    sigma gst h = Some st ->
+    succ_list_leading_failed_nodes (failed_nodes gst) (succ_list st) = 0.
+Proof.
+  unfold total_leading_failed_nodes in *.
+  intros.
+
+  assert (In h (live_nodes gst)).
+  {
+    unfold live_nodes.
+    apply filter_In.
+    split.
+    - live_addr_inv; easy.
+    - now apply Coqlib.proj_sumbool_is_true.
+  }
+
+  assert (exists n, maybe_count_failed_nodes gst h = Some n).
+  {
+    unfold maybe_count_failed_nodes.
+    find_rewrite.
+    eexists; eauto.
+  }
+  break_exists_name failed_succs.
+
+  replace failed_succs with 0 in *.
+  - eapply maybe_count_failed_nodes_Some; eauto.
+  - symmetry.
+    eapply sum_of_nats_zero_means_all_zero; eauto.
+    eapply FilterMap.filterMap_In; eauto.
+Qed.
+
+Definition zero_total_leading_failed_nodes (gst : global_state) : Prop :=
+  total_leading_failed_nodes gst = 0.
+
+Theorem zero_leading_failed_nodes_implies_all_first_succs_best :
+  forall gst,
+    reachable_after_churn gst ->
+    (* total leading failed nodes says nothing about the length of successor lists *)
+    nonempty_succ_lists gst ->
+    zero_total_leading_failed_nodes gst ->
+    all_first_succs_best gst.
+Proof.
+  unfold all_first_succs_best, first_succ_is_best_succ, zero_total_leading_failed_nodes.
+  intros.
+  find_eapply_lem_hyp live_inv;
+    break_and;
+    break_exists_exists.
+  unfold nonempty_succ_lists in *.
+  find_copy_apply_hyp_hyp.
+  destruct (succ_list _) as [| p rest] eqn:?H; [congruence|].
+  exists p. exists rest.
+  repeat split; auto.
+
+  assert (live gst h) by eauto using live_intro.
+  find_copy_apply_lem_hyp live_live_addr.
+  find_rewrite_lem live_live_addr.
+  find_copy_apply_lem_hyp zero_failed_nodes_total_implies_zero_locally; auto.
+  eapply zero_leading_failed_nodes_best_succ; eauto.
+  eapply live_node_characterization; eauto.
+  eapply nonempty_succ_lists_always_belong_to_joined_nodes; eauto.
+Qed.
+
+Lemma always_reachable_after_churn :
+  forall ex,
+    reachable_st (occ_gst (infseq.hd ex)) ->
+    infseq.always (lift_gpred_to_ex reachable_after_churn) ex.
+Proof.
+Admitted.
+
+Lemma zero_leading_failed_all_best :
+    forall gst,
+      reachable_after_churn gst ->
+      (gpred_and
+         nonempty_succ_lists
+         zero_total_leading_failed_nodes) gst ->
+      all_first_succs_best gst.
+Proof.
+  unfold gpred_and.
+  intros.
+  break_and.
+  auto using zero_leading_failed_nodes_implies_all_first_succs_best.
+Qed.
+
+Theorem continuously_zero_total_leading_failed_nodes_implies_phase_one :
+  forall ex,
+    reachable_st (occ_gst (infseq.hd ex)) ->
+    infseq.continuously (infseq.and_tl
+                           (lift_gpred_to_ex zero_total_leading_failed_nodes)
+                           (lift_gpred_to_ex nonempty_succ_lists))
+                        ex ->
+    phase_one ex.
+Proof.
+Admitted.
+
+(* Partial order on successor lists for proving phase two *)
+Inductive succ_list_improved (failed : list addr) : list pointer -> list pointer -> Prop :=
+| succ_list_improved_refl :
+    forall succs,
+      succ_list_improved failed succs succs
+| succ_list_improved_drop_dead :
+    forall h rest,
+      In (addr_of h) failed ->
+      succ_list_improved failed (h :: rest) rest.
+
+(* Lifting succ_list_improved to be a sensible order on global states *)
+Definition succ_lists_some_improved (gst gst' : global_state) :=
+  nodes gst = nodes gst' /\
+  failed_nodes gst = failed_nodes gst' /\
+  exists h st st',
+    sigma gst h = Some st ->
+    sigma gst' h = Some st' ->
+    succ_list_improved (failed_nodes gst) (succ_list st) (succ_list st').
 
 Definition correct_pred (gst : global_state) (h : pointer) (p : option pointer) : Prop :=
   exists p0,
@@ -67,7 +537,7 @@ Definition correct_pointers gst :=
 Definition phase_two (ex : infseq.infseq occurrence) :=
   lb_execution ex ->
   reachable_st (occ_gst (infseq.hd ex)) ->
-  eventually_always_net correct_pointers ex.
+  infseq.continuously (lift_gpred_to_ex correct_pointers) ex.
 
 Definition ideal (gst : global_state) : Prop :=
   forall h st,
@@ -91,4 +561,3 @@ Theorem chord_stabilization :
          (fun ex' => (ideal (occ_gst (infseq.hd ex')))))
       ex.
 Admitted.
-
